---
title: "Expected numbers of full and half-sibling pairs between surveys"
author: "Robin Aldridge-Sutton"
output:
  html_document:
    toc: true
---

```{r setup, include=FALSE}
knitr::opts_chunk$set(echo = TRUE)
```

### Full-sibling pairs

## Younger animal alive at time of first sample

$$ 2 E(FSP_{t_1}) \phi^{t_2 - t_1} $$

### Younger animal born between sample-times

If an animal $j$ is born at a time $b_2$ such that $t_1 < b_2 \le t_2$, then there is an FSP between $t_1$ and $t_2$ for each animal $i$ that is born at a time $b_1$ before $t_1$, so that $b_1 < t_1$, and survives until $t_1$, and has a mother that survives until $b_2$, and gives birth to $j$ then, and a father that survives to $b_2 - 1$ and conceives $j$ then, given $j$ survives to $t_2$.

The probability that $i$ survives to $t_1$ is $\phi^{t_1 - b_1}$.

The probability that the mother survives from $b_1$ to $b_2$ is $\phi^{b_2 - b_1}$.

The probability that the mother has another calf at $b_2$, given that she survives until then, is $\beta$.

The probability that the father survives from $b_1 - 1$ to $b_2 - 1$ is $\phi^{b_2 - 1 - (b_1 - 1)} = \phi^{b_2 - b_1}$.

The probability that the father conceives a calf at $b_2 - 1$, given that he survives until then, is $\frac{1}{M^*_{b_2-1}}$.

The probability that this calf survives to time $t_2$ is $\phi^{t_2 - b_2}$.

For each animal born at time $b_1$ the probability that it forms a pair such as $i$ and $j$ is then 
$$\phi^{t_1 - b_1} \phi^{b_2 - b_1} \beta \phi^{b_2 - b_1} \frac{1}{M^*_{b_2-1}} \phi^{t_2 - b_2} = \frac{\beta \phi^{t_1 + t_2 + b_2 - 3 b_1}}{M^*_{b_2-1}}.$$

Let $FSP_{t_1, t_2, b_1, b_2}$ be the number of pairs such as $i$ and $j$.  Then
$$FSP_{t_1, t_2, b_1, b_2} \sim Bin \left( B_{b_1}, \frac{\beta \phi^{t_1 + t_2 + b_2 - 3 b_1}}{M^*_{b_2-1}} \right),$$
and following the same reasoning as above
$$E(FSP_{t_1, t_2, b_1, b_2}) = E(B_{b_1}) \frac{\beta \phi^{t_1 + t_2 + b_2 - 3 b_1}}{M^*_{b_2-1}}$$
$$= E(N_{b_1}) \left(1 - \frac{\phi}{\lambda}\right) \frac{\beta \phi^{t_1 + t_2 + b_2 - 3 b_1}}{M^*_{b_2-1}}$$
$$= E(N_{b_1}) \left(1 - \frac{\phi}{\lambda}\right) \frac{\beta \phi^{t_1 + t_2 + b_2 - 3 b_1}}{\frac{E(N_{b_2})}{2}\left(\frac{\phi}{\lambda}\right)^\alpha \phi^{-1}}$$
$$= 2 \beta \frac{E(N_{b_1})}{E(N_{b_2})} \left(1 - \frac{\phi}{\lambda}\right) \left(\frac{\lambda}{\phi}\right)^\alpha \phi^{t_1 + t_2 + b_2 - 3 b_1 + 1}$$

$$E \left( \sum_{b_1 \le t_1}\sum_{t_1 < b_2 \le t_2}FSP_{t_1, t_2, b_1, b_2} \right) = \sum_{b_1 \le t_1}\sum_{t_1 < b_2 \le t_2}E(FSP_{t_1, t_2, b_1, b_2})$$
$$= \sum_{b_1 \le t_1}\sum_{t_1 < b_2 \le t_2} 2 \beta \frac{E(N_{b_1})}{E(N_{b_2})} \left(1 - \frac{\phi}{\lambda}\right) \left(\frac{\lambda}{\phi}\right)^\alpha \phi^{t_1 + t_2 + b_2 - 3 b_1 + 1}$$
$$= 2 \beta \left(1 - \frac{\phi}{\lambda}\right) \left(\frac{\lambda}{\phi}\right)^\alpha \phi^{t_1 + t_2 + 1} \sum_{b_1 \le t_1}\sum_{t_1 < b_2 \le t_2}\frac{E(N_{t_2}) \lambda^{t_2 - b_2}}{E(N_{t_2})\lambda^{t_2 - b_1}} \phi^{b_2 - 3 b_1}$$
$$= 2 \beta \left(1 - \frac{\phi}{\lambda}\right) \left(\frac{\lambda}{\phi}\right)^\alpha \phi^{t_1 + t_2 + 1} \sum_{b_1 \le t_1}\sum_{t_1 < b_2 \le t_2} \lambda^{b_1 - b_2} \phi^{b_2 - 3 b_1}$$
$$\sum_{b_1 \le t_1}\sum_{t_1 < b_2 \le t_2} \lambda^{b_1 - b_2} \phi^{b_2 - 3 b_1} = \sum_{b_1 \le t_1}\sum_{t_1 < b_2 \le t_2} \left( \frac{\phi}{\lambda} \right)^{b_2 - b_1} \phi^{-2 b_1}$$
$$= \sum_{b_1 \le t_1} \left( \frac{\phi}{\lambda} \right)^{-b_1} \phi^{-2 b_1} \sum_{t_1 < b_2 \le t_2} \left( \frac{\phi}{\lambda} \right)^{b_2}$$
$$= \sum_{b_1 \le t_1} \left( \frac{\phi^3}{\lambda} \right)^{-b_1} \sum_{t_1 < b_2 \le t_2} \left( \frac{\phi}{\lambda} \right)^{b_2}$$
$$= \left\{\left( \frac{\phi^3}{\lambda} \right)^{-t_1} + \left( \frac{\phi^3}{\lambda} \right)^{-(t_1 - 1)} + ... \right\} \frac{\left( \frac{\phi}{\lambda} \right)^{t_1 + 1} - \left( \frac{\phi}{\lambda} \right)^{t_2 + 1}}{1 - \left( \frac{\phi}{\lambda} \right)}$$
$$= \left\{ \frac{\left( \frac{\phi^3}{\lambda} \right)^{-t_1}}{1 - \left( \frac{\phi^3}{\lambda} \right)} \right\} \left\{ \frac{\left( \frac{\phi}{\lambda} \right)^{t_1 + 1} - \left( \frac{\phi}{\lambda} \right)^{t_2 + 1}}{1 - \left( \frac{\phi}{\lambda} \right)} \right\}$$
$$= \frac{\left( \frac{\phi}{\lambda} \right)^{t_1 + 1} - \left( \frac{\phi}{\lambda} \right)^{t_2 + 1}}{\left( \frac{\phi^3}{\lambda} \right)^{t_1} \left\{ 1 - \left( \frac{\phi^3}{\lambda} \right)\right\} \left\{1 - \left( \frac{\phi}{\lambda} \right) \right\}}$$
$$E(FSP_{t_1, t_2}) = 2 \beta \left(1 - \frac{\phi}{\lambda}\right) \left(\frac{\lambda}{\phi}\right)^\alpha \phi^{t_1 + t_2 + 1} \frac{\left( \frac{\phi}{\lambda} \right)^{t_1 + 1} - \left( \frac{\phi}{\lambda} \right)^{t_2 + 1}}{\left( \frac{\phi^3}{\lambda} \right)^{t_1} \left\{ 1 - \left( \frac{\phi^3}{\lambda} \right)\right\} \left\{1 - \left( \frac{\phi}{\lambda} \right) \right\}}$$


